the new scope is 5 to 6 times faster

orchestrator/Scope.v
@@ -1,4 +1,12 @@
 From Ltac2 Require Import Ltac2.
+
+Require Import ZArith.
+Require Import PArith.BinPos.
+Require Import SMTCoq.bva.BVList.
+Require Import NArith.BinNatDef.
+
+From SMTCoq Require Import SMT_classes SMT_classes_instances.
+
 From Trakt Require Import Trakt.
 
 From Sniper Require Import definitions.
@@ -10,6 +18,7 @@ From Sniper Require Import case_analysis.
 From Sniper Require Import higher_order.
 From Sniper Require Import anonymous_functions.
 From Sniper Require Import instantiate.
+From Sniper Require Import Sniper.
 
 Require Import Tactics.
 Require Import Triggers.
@@ -33,38 +42,310 @@ Ltac2 scope_triggers () :=
    trigger_generation_principle;
    trigger_polymorphism ()].
 
+Ltac2 init_triggered ():=
+[("my_get_def", [constr:(Z.add)]);
+("my_get_def", [constr:(Z.sub)]);
+("my_get_def", [constr:(Z.mul)]);
+("my_get_def", [constr:(Z.eqb)]);
+("my_get_def", [constr:(Z.ltb)]);
+("my_get_def", [constr:(Z.leb)]);
+("my_get_def", [constr:(Z.geb)]);
+("my_get_def", [constr:(Z.gtb)]);
+("my_get_def", [constr:(Z.lt)]);
+("my_get_def", [constr:(Z.le)]);
+("my_get_def", [constr:(Z.ge)]);
+("my_get_def", [constr:(Z.gt)]);
+("my_get_def", [constr:(Pos.lt)]);
+("my_get_def", [constr:(Pos.le)]);
+("my_get_def", [constr:(Pos.ge)]);
+("my_get_def", [constr:(Pos.gt)]);
+("my_get_def", [constr:(Z.to_nat)]);
+("my_get_def", [constr:(Pos.mul)]);
+("my_get_def", [constr:(Pos.add)]);
+("my_get_def", [constr:(Pos.sub)]);
+("my_get_def", [constr:(Init.Nat.add)]);
+("my_get_def", [constr:(Init.Nat.mul)]);
+("my_get_def", [constr:(Nat.eqb)]);
+("my_get_def", [constr:(Nat.leb)]);
+("my_get_def", [constr:(Nat.ltb)]);
+("my_get_def", [constr:(Peano.lt)]);
+("my_get_def", [constr:(ge)]); 
+("my_get_def", [constr:(gt)]);
+("my_get_def", [constr:(N.add)]);
+("my_get_def", [constr:(N.mul)]);
+("my_get_def", [constr:(N.eqb)]);
+("my_get_def", [constr:(N.leb)]);
+("my_get_def", [constr:(N.ltb)]);
+("my_get_def", [constr:(Peano.lt)]);
+("my_get_def", [constr:(ge)]); ("my_get_def", [constr:(gt)]);
+("my_get_def", [constr:(negb)]);
+("my_get_def", [constr:(not)]);
+("my_get_def", [constr:(andb)]);
+("my_get_def", [constr:(orb)]);
+("my_get_def", [constr:(implb)]);
+("my_get_def", [constr:(xorb)]);
+("my_get_def", [constr:(Bool.eqb)]);
+("my_get_def", [constr:(iff)]);
+("my_get_def", [constr:(BITVECTOR_LIST.bv_eq)]);
+("my_get_def", [constr:(BITVECTOR_LIST.bv_and)]);
+("my_get_def", [constr:(BITVECTOR_LIST.bv_or)]);
+("my_get_def", [constr:(BITVECTOR_LIST.bv_xor)]);
+("my_get_def", [constr:(BITVECTOR_LIST.bv_add)]);
+("my_get_def", [constr:(BITVECTOR_LIST.bv_mult)]);
+("my_get_def", [constr:(BITVECTOR_LIST.bv_ult)]);
+("my_get_def", [constr:(BITVECTOR_LIST.bv_slt)]);
+("my_get_def", [constr:(BITVECTOR_LIST.bv_concat)]);
+("my_get_def", [constr:(BITVECTOR_LIST.bv_shl)]);
+("my_get_def", [constr:(BITVECTOR_LIST.bv_shr)]);
+("my_get_def", [constr:(@FArray.select)]);
+("my_get_def", [constr:(@FArray.diff)]);
+("my_get_def", [constr:(is_true)]);
+("my_get_def", [constr:(@eqb_of_compdec)]);
+("my_get_def", [constr:(CompDec)]);
+("my_get_def", [constr:(Nat_compdec)]);
+("my_get_def", [constr:(list_compdec)]);
+("my_get_def", [constr:(prod_compdec)]);
+("my_get_def", [constr:(Z_compdec)]);
+("my_algebraic_types", [constr:(Z)]);
+("my_algebraic_types", [constr:(bool)]);
+("my_algebraic_types", [constr:(positive)]);
+("my_algebraic_types", [constr:(N)]);
+("my_algebraic_types", [constr:(nat)]);
+("my_algebraic_types", [constr:(EqbType)]);
+("my_algebraic_types", [constr:(@CompDec)]);
+("my_algebraic_types", [constr:(Comparable)]);
+("my_algebraic_types", [constr:(Inhabited)]);
+("my_algebraic_types", [constr:(OrderedType.Compare)])].
+
 Ltac my_get_def t := get_def t.
 
-(* Ltac my_trakt_bool := trakt bool. *)
+Ltac my_trakt_bool := revert_all ; trakt bool ; intros.
 
 Ltac my_higher_order_equalities H := expand_hyp H ; clear H.
+
+Ltac my_higher_order := prenex_higher_order.
 
 Ltac my_fixpoints H := eliminate_fix_hyp H.
 
 Ltac my_pattern_matching H := eliminate_dependent_pattern_matching H.
 
-(* Ltac my_anonymous_functions := anonymous_funs. *)
+Ltac my_anonymous_functions := anonymous_funs.
 
 Ltac my_algebraic_types t := try (interp_alg_types t).
 
 Ltac my_gen_principle t := pose_gen_statement t.
 
+Ltac my_gen_principle_temporary := ltac2:(get_projs_in_variables 'prod_types).
+
 Ltac my_polymorphism := elimination_polymorphism.
 
-(* [(* "my_trakt_bool"; TODO *) "my_get_def"; 
-"my_higher_order_equalities"; "my_fixpoints" ; "my_pattern_matching"; (* "my_anonymous_functions"; *)
-"my_algebaraic_types"; "my_gen_principle"; "my_polymorphism"] *)
+Ltac2 trigger_generation_principle :=
+  (TContains (TSomeHyp, NotArg) (TInd None (NotArg))).
 
-
-Ltac2 scope () := orchestrator 10 [trigger_definitions; trigger_higher_order_equalities; 
-trigger_fixpoints; trigger_pattern_matching; trigger_algebraic_types; trigger_polymorphism ()] ["my_get_def"; "my_higher_order_equalities"; "my_fixpoints";
-"my_pattern_matching"; "my_algebraic_types"; "my_polymorphism"] { triggered_tacs := [] }.
+Ltac2 scope () := orchestrator 5 
+[trigger_anonymous_funs () ; trigger_higher_order ; 
+trigger_definitions; trigger_higher_order_equalities; 
+trigger_fixpoints; trigger_pattern_matching; 
+trigger_algebraic_types; trigger_polymorphism (); 
+trigger_generation_principle ; trigger_trakt_bool ()] 
+["my_anonymous_functions" ; "my_higher_order"; 
+"my_get_def"; "my_higher_order_equalities"; 
+"my_fixpoints"; "my_pattern_matching"; 
+"my_algebraic_types"; "my_polymorphism"; 
+"my_gen_principle_temporary" ; "my_trakt_bool"] { triggered_tacs := (init_triggered ()) }.
 
 Tactic Notation "scope" := ltac2:(scope ()).
 
-Lemma toto A : length (@nil A) = 0.
+Local Open Scope Z_scope.
+
+(** Examples on lists *)
+
+(* A simple example *)
+Goal forall (l : list Z) (x : Z), hd_error l = Some x -> (l <> nil).
 Proof.
-Time scope.
+Time scope; verit. (* Finished transaction in 0.507 secs (0.471u,0.01s) (successful) *)
+Undo.
+Time snipe. (* Finished transaction in 2.783 secs (2.428u,0.007s) (successful) *)
+Qed.
+
+Section Generic.
+
+  Variable (A : Type).
+  Hypothesis HA : CompDec A.
+  Goal forall (l : list A) (x : A),  hd_error l = Some x -> (l <> nil).
+  Proof.
+  Time scope; verit. (* Finished transaction in 0.549 secs (0.516u,0.s) (successful) *)
+  Undo.
+  Time snipe. (* Finished transaction in 3.028 secs (2.64u,0.015s) (successful) *)
+  Qed.
+
+End Generic.
+
+Require Import List.
+Import ListNotations.
+
+Section destruct_auto.
+
+  Variable A : Type.
+  Variable HA : CompDec A.
+
+Theorem app_eq_unit_auto :
+    forall (x y: list A) (a:A),
+      x ++ y = a :: nil -> x = [] /\ y = [a] \/ x = [a] /\ y = [].
+  Proof.
+  Time intros ; scope; verit. (* Finished transaction in 1.781 secs (1.144u,0.007s) (successful) *)
+  Undo.  
+  Time snipe. (*Finished transaction in 5.66 secs (4.35u,0.006s) (successful) *) Qed.
+
+
+End destruct_auto.
+
+Require Import Bool.
+
+
+(* Example of searching an element in a list *)
+Fixpoint search {A : Type} {H: CompDec A} (x : A) l :=
+  match l with
+  | [] => false
+  | x0 :: l0 => eqb_of_compdec H x x0 || search x l0
+  end.
+
+(* (* The proof of this lemma, except induction, can be automatized *)
+Lemma search_app_snipe : forall {A: Type} {H : CompDec A} (x: A) (l1 l2: list A),
+    search x (l1 ++ l2) = ((search x l1) || (search x l2))%bool.
+Proof. intros A H x l1 l2. 
+Time induction l1 as [ | x0 l0 IH]; simpl; ltac2:(Control.enter (fun () => scope ())) ; verit.
+Time induction l1 as [ | x0 l0 IH]; simpl; snipe (* Finished transaction in 9.089 secs (7.921u,0.005s) (successful). *)
+
+Qed. TODO => fixpoints never stops for some reason *)
+
+Lemma search_app : forall {A: Type} {H : CompDec A} (x: A) (l1 l2: list A),
+    search x (l1 ++ l2) = ((search x l1) || (search x l2))%bool.
+Proof.
+  intros A H x l1 l2. induction l1 as [ | x0 l0 IH].
+  - reflexivity.
+  - simpl. destruct (eqb_of_compdec H x x0).
+    + reflexivity.
+    + rewrite IH. reflexivity.
+Qed.
+
+(* It can be fully automatized *)
+Lemma snipe_search_lemma : forall (A : Type) (H : CompDec A) (x: A) (l1 l2 l3: list A),
+search x (l1 ++ l2 ++ l3) = search x (l3 ++ l2 ++ l1).
+Proof. intros A H. 
+
+Time snipe @search_app. (* Finished transaction in 5.777 secs (5.007u,0.s) (successful) *)
+Undo.
+pose proof search_app.
+Time scope; verit. (* Finished transaction in 0.842 secs (0.76u,0.007s) (successful) *)
+
+
+Qed.
+
+
+(* Another example with search *)
+Lemma in_inv : forall (A: Type) (HA : CompDec A) (a b:A) (l:list A),
+    search b (a :: l) -> eqb_of_compdec HA a b \/ search b l.
+Proof. intros A HA.  
+Time snipe. (* Finished transaction in 2.652 secs (2.239u,0.s) (successful) *)
+Undo.
+Time scope; verit. (* Finished transaction in 0.434 secs (0.405u,0.s) (successful) *)
+
+Qed.
+
+
+(* Another example with an induction *)
+Lemma app_nil_r : forall (A: Type) (H: CompDec A) (l:list A), (l ++ [])%list = l.
+Proof. 
+ intros A H. Time induction l; snipe. (* Finished transaction in 4.195 secs (3.601u,0.s) (successful) *)
+Undo.
+Time induction l ; ltac2:(Control.enter (fun () => scope ())) ; verit. 
+(* Finished transaction in 0.952 secs (0.902u,0.s) (successful) *)
+
+Qed.
+
+Section higher_order.
+
+
+Variable A B C: Type.
+Variable HA : CompDec A.
+Variable HB : CompDec B.
+Variable HC : CompDec C.
+
+Fixpoint zip {A B : Type} (l : list A) (l' : list B) :=
+  match l, l' with
+  | [], _ => []
+  | x :: xs, [] => []
+  | x :: xs, y :: ys => (x, y) :: zip xs ys 
+  end.
+
+(*
+(* A nice example but a bit slow ~70s: we should investigate to improve the performance *)
+
+Lemma zip_map : forall (f : A -> B) (g : A -> C) (l : list A),
+map (fun (x : A) => (f x, g x)) l = zip (map f l) (map g l).
+Proof. (* Time intros f g l ; induction l; snipe2.  *)
+Time intros f g l ; induction l ; ltac2:(Control.enter (fun () => scope ())) ; verit.
+
+Qed. TODO *)
+
+(* 
+TODO no applicable 
+
+An example with higher order and anonymous functions 
+Note that as map should be instantiated by f and g, 
+it does not work by using an induction principle which generalizes 
+on f and g, so f and g have to be introduced before l 
+It also work only with snipe2 because the arrow type instances will 
+make SMTCoq complain 
+Lemma map_compound : forall (f : A -> B) (g : B -> C) (l : list A), 
+map g (map f l) = map (fun x => g (f x)) l.
+Proof.
+Time induction l; snipe2. (* Finished transaction in 17.149 secs (15.047u,0.08s) (successful) *)
+Undo.
+(* Time induction l; ltac2:(Control.enter (fun () => scope ())) ; verit. *)
+Abort. *)
+End higher_order.
+
+From Sniper Require Import tree.
+
+(** Examples on trees *)
+
+Lemma empty_tree_Z2 : forall (t : @tree Z) a t' b,
+is_empty t = true -> t <> Node a t' b.
+Proof. Time intros t a t' b; snipe. (* 2.752 s *)
+Undo.
+Time intros t a t' b ; ltac2:(Control.enter (fun () => scope ())) ; verit.
+(* Finished transaction in 0.785 secs (0.754u,0.s) (successful) *)
+Qed.
+
+(* TODO try with the other elim poly strat Lemma rev_elements_app :
+ forall A (H:CompDec A) s acc, tree.rev_elements_aux A acc s = ((tree.rev_elements A s) ++ acc)%list.
+Proof. intros A H s ; induction s.
+- Time snipe app_nil_r. (* Finished transaction in 8.973 secs (7.871u,0.007s) (successful) *)
+Undo. pose proof List.app_nil_r. Time scope; verit.
+- snipe (app_ass, app_nil_r).
+Qed.
+ *)
+
+Lemma rev_elements_app :
+ forall A (H:CompDec A) s acc, tree.rev_elements_aux A acc s = ((tree.rev_elements A s) ++ acc)%list.
+Proof. intros A H s ; induction s.
+- snipe app_nil_r.
+- snipe (app_ass, app_nil_r).
+Qed.
+
+
+Lemma rev_elements_node c (H: CompDec c) l x r :
+ rev_elements c (Node l x r) = (rev_elements c r ++ x :: rev_elements c l)%list.
+Proof. Time snipe (rev_elements_app, app_nil_r). 
+(* Finished transaction in 11.955 secs (10.477u,0.007s) (successful) *)
+Undo.
+pose proof rev_elements_app.
+pose proof app_nil_r.
+Fail scope; verit. Abort.
+
+
 
 
 
